cerberus-heaplang/CerberusHeapLang/Potential.lean
@@ -104,8 +104,10 @@ theorem Frag.esize_le_pot {e : CoreExpr} (hf : Frag e) : esize e ≤ pot e := by
   | store => simp [esize, pot, storeRedex]
   | load => simp [esize, pot, loadRedex]
   | create => simp [esize, pot, createRedex]
-  | kill hstatic => simp [esize, pot, killRedex]
-  | kill_op hstatic hnvK hpK hdK => simp [esize, pot, killOpRedex]
+  | kill => simp [esize, pot, killRedex]
+  | kill_op hnvK hpK hdK => simp [esize, pot, killOpRedex]
+  | alloc => simp [esize, pot, allocRedex]
+  | alloc_op hnvA hp1 hp2 hd1 hd2 => simp [esize, pot, allocOpRedex]
   | sseq hf1 hf2 ih1 ih2 => simp only [esize_sseq, pot_sseq]; omega
   | annot hfb ihb => simp only [esize_annot, pot_annot]; omega
   | save hp hd hb ih =>
@@ -144,8 +146,10 @@ theorem Frag.pot_le_two {e : CoreExpr} (hf : Frag e) : pot e ≤ 2 * esize e := 
   | store => simp [esize, pot, storeRedex]
   | load => simp [esize, pot, loadRedex]
   | create => simp [esize, pot, createRedex]
-  | kill hstatic => simp [esize, pot, killRedex]
-  | kill_op hstatic hnvK hpK hdK => simp [esize, pot, killOpRedex]
+  | kill => simp [esize, pot, killRedex]
+  | kill_op hnvK hpK hdK => simp [esize, pot, killOpRedex]
+  | alloc => simp [esize, pot, allocRedex]
+  | alloc_op hnvA hp1 hp2 hd1 hd2 => simp [esize, pot, allocOpRedex]
   | sseq hf1 hf2 ih1 ih2 => simp only [esize_sseq, pot_sseq]; omega
   | annot hfb ihb => simp only [esize_annot, pot_annot]; omega
   | save hp hd hb ih =>
@@ -207,18 +211,30 @@ theorem Frag.pot_step_bound {M : MachineCtx} {e : CoreExpr} {ρ : EnvStack}
       simpa [Prod.mk.injEq] using hout
     subst h1
     left; simp [pot, createRedex]
-  | kill hstatic =>
+  | kill =>
     obtain ⟨σ'', hmem, hout⟩ := hs.kill_inv
     obtain ⟨h1, -, -⟩ : e' = _ ∧ ρ' = ρ ∧ σ' = σ'' := by
       simpa [Prod.mk.injEq] using hout
     subst h1
     left; simp [pot, killRedex]
-  | kill_op hstatic hnvK hpK hdK =>
+  | kill_op hnvK hpK hdK =>
     obtain ⟨pv, -, hout⟩ := hs.kill_op_inv hnvK
     obtain ⟨h1, -, -⟩ : e' = _ ∧ ρ' = ρ ∧ σ' = σ := by
       simpa [Prod.mk.injEq] using hout
     subst h1
     left; simp [pot, killOpRedex]
+  | alloc =>
+    obtain ⟨pv, σ'', hmem, hout⟩ := hs.alloc_inv
+    obtain ⟨h1, -, -⟩ : e' = _ ∧ ρ' = ρ ∧ σ' = σ'' := by
+      simpa [Prod.mk.injEq] using hout
+    subst h1
+    left; simp [pot, allocRedex]
+  | alloc_op hnvA hp1 hp2 hd1 hd2 =>
+    obtain ⟨al, sz, -, -, hout⟩ := hs.alloc_op_inv hnvA
+    obtain ⟨h1, -, -⟩ : e' = _ ∧ ρ' = ρ ∧ σ' = σ := by
+      simpa [Prod.mk.injEq] using hout
+    subst h1
+    left; simp [pot, allocOpRedex]
   | sseq hf1 hf2 ih1 ih2 =>
     rcases hs.sseq_inv with ⟨e1', ρ'', σ'', hnj, hstep, hout⟩ |
         ⟨_, _, v, _, _, _, he1, _, hout⟩ | ⟨_, _, ds', v, _, _, _, he1, _, hout⟩ |
